Lampe/Lampe/Tactic/Steps.lean
@@ -87,8 +87,10 @@ def getClosingTerm (val : Expr) : TacticM (Option (TSyntax `term × Bool)) := wi
         | ``Lampe.Builtin.fMul => return some (←``(genericTotalPureBuiltin_intro Builtin.fMul rfl (a := ())), true)
         | ``Lampe.Builtin.fSub => return some (←``(genericTotalPureBuiltin_intro Builtin.fSub rfl (a := ())), true)
         | ``Lampe.Builtin.fNeg => return some (←``(genericTotalPureBuiltin_intro Builtin.fNeg rfl (a := ())), true)
+        | ``Lampe.Builtin.fDiv => return some (←``(fDiv_intro), false)
 
         | ``Lampe.Builtin.fEq => return some (←``(genericTotalPureBuiltin_intro Builtin.fEq rfl (a := ())), true)
+        | ``Lampe.Builtin.uEq => return some (←``(genericTotalPureBuiltin_intro Builtin.uEq rfl), true)
 
         | ``Lampe.Builtin.uAdd => return some (←``(uAdd_intro), false)
 
@@ -313,9 +315,15 @@ lemma STHoare.pluck_pures : (P → STHoare lp Γ H e Q) → (STHoare lp Γ (P �
   intro h
   simp_all [STHoare, THoare, SLP.pure_star_iff_and]
 
-syntax "loop_inv" term : tactic
-elab "loop_inv" inv:term : tactic => do
-  let goals ← steps (← getMainGoal) 1 [←``(loop_inv_intro $inv)]
+theorem bindVar {v : α} { P : α → Prop } (hp: ∀v, P v) : P v := by
+  apply hp v
+
+-- syntax "loop_inv" term : tactic
+elab "loop_inv" n:optional(ident) ("=>")? inv:term : tactic => do
+  let solver ← match n with
+  | some n => ``(bindVar (fun $n => (loop_inv_intro $inv)))
+  | none => ``(loop_inv_intro $inv)
+  let goals ← steps (← getMainGoal) 1 [solver]
   replaceMainGoal goals
 
 theorem callDecl_direct_intro {p} {Γ : Env} {func} {args} {Q H}
@@ -367,9 +375,6 @@ theorem callTrait_direct_intro {impls : List $ Lampe.Ident × Function}
 
 syntax "enter_trait" "[" term,* "]" term  : tactic
 macro_rules | `(tactic|enter_trait [$generics,*] $envSyn) => `(tactic|apply callTrait_direct_intro (by try_impls_all [$generics,*] $envSyn) (by rfl) (by rfl) (by rfl) (by rfl))
-
-theorem bindVar {v : α} { P : α → Prop } (hp: ∀v, P v) : P v := by
-  apply hp v
 
 theorem enter_block H Q : STHoare p Γ H e Q → STHoare p Γ H e Q := by simp
 
